src/Model.v
@@ -5,25 +5,48 @@ Require Import
   Coq.Program.Program
   Coq.Sets.Classical_sets
   Coq.Sets.Ensembles
+  Coq.Unicode.Utf8
   Same_set
   Stream
   LTL.
 
-(*
 Module StreamLTL <: LinearTemporalLogic.
 
 Variable a : Type.
 
 Definition t := Ensemble (Stream a).
 
-Definition equiv := Same_set (Stream a).
-Definition not := Complement (Stream a).
-Definition and := Intersection (Stream a).
-Definition or := Union (Stream a).
+Definition not   := Complement (Stream a).
+Definition or    := Union (Stream a).
+Definition true  := Full_set (Stream a).
+Definition false := Empty_set (Stream a).
+Definition and   := Intersection (Stream a).
+Definition impl  := Included (Stream a).
+Definition eqv   := Same_set (Stream a).
 
-Definition next (p : t) : t := fun s => p (from 1 s).
-Definition until (p q : t) : t :=
-  fun s => exists i, q (from i s) /\ forall k, k < i -> p (from k s).
+Program Instance impl_reflexive : Reflexive impl.
+Next Obligation.
+  unfold impl.
+  now repeat intro.
+Qed.
+Program Instance impl_transitive : Transitive impl.
+Next Obligation.
+  unfold impl, Included in *.
+  repeat intro.
+  now intuition.
+Qed.
+
+Instance eqv_equivalence : Equivalence eqv.
+Proof.
+  split.
+  - intro x; now split.
+  - repeat intro; split; destruct H; now intuition.
+  - repeat intro; split; destruct H, H0; now transitivity y.
+Defined.
+
+Definition next : t -> t :=
+  λ p s, (s, 1) ⊨ p.
+Definition until : t -> t -> t :=
+  λ p q s, ∃ i, (s, i) ⊨ q /\ ∀ k, k < i -> (s, k) ⊨ p.
 
 End StreamLTL.
-*)
